proofs refactored and some comments added

LeftistHeap.v
@@ -8,24 +8,29 @@ From Equations Require Import Equations.
 
 Open Scope order_scope.
 
-Lemma snd_true a b : a || true || b.
-Proof.
-by case: a.
-Qed.
+Lemma snd_true3 a b : a || true || b.
+Proof. by case: a. Qed.
 
-Lemma trd_true a b : b || a || true.
-Proof.
-by case: a; case b.
-Qed.
-Hint Resolve trd_true snd_true lexx : core.
+Lemma trd_true3 a b : b || a || true.
+Proof. by case: a; case b. Qed.
+
+Lemma snd_true2 a : a || true.
+Proof. by case: a. Qed.
+
+Lemma add_lt_le a b c d: (a < c)%N -> (b <= d)%N -> (a + b < c + d)%N.
+Proof. by move=> *; rewrite [a + b]addnC -ltn_subRL -addnBA // ltn_addr. Qed.
+
+Lemma add_le_lt a b c d: (a <= c)%N -> (b < d)%N -> (a + b < c + d)%N.
+Proof. move=> *; rewrite [a + b]addnC [c + d]addnC. by apply: add_lt_le. Qed.
+
+
+Hint Resolve trd_true3 snd_true3 snd_true2 lexx ltxx : core.
 
 Module leftistheap.
-(*Leftist heaps are heap-ordered binary trees that satisfy the
-leftist property: the rank of any left child is at least as large as the rank of its
-right sibling. The rank of a node is defined to be the length of its right spine
-(i.e., the rightmost path from the node in question to an empty node). A simple
-consequence of the leftist property is that the right spine of any node is always
-the shortest path to an empty node.*)
+(* Leftist heaps are heap-ordered binary trees that satisfy the                         *)
+(* leftist property: the rank of any left child is at least as large as the rank of its *)
+(* right sibling. The rank of a node is defined to be the length of its right spine     *)
+(* (i.e., the rightmost path from the node in question to an empty node).               *)
 Section LeftistDef.
 Variables (T: ordType).
 
@@ -39,6 +44,7 @@ Arguments Emp {T}.
 Notation "[ tl | n , x | tr ]" := (Node n x tl tr) (at level 0).
 Notation "'[||]'" := Emp.
 
+(* Definition of arbitrary measure on Heaps *)
 Module Measure.
 Structure mixin_of {T : ordType} (measure : heap T -> nat) :=
   Mixin {
@@ -80,6 +86,13 @@ Export Measure.Exports.
 Variables (T : ordType).
 Implicit Type h : heap T.
 
+Definition empty h :=
+if h is Emp then true else false.
+
+Theorem emptyP h : reflect (h = Emp) (empty h).
+Proof. case h; by constructor. Qed.
+
+(* Definition of decidable equality on Heaps  *)
 Fixpoint eqheap h1 h2 :=
   match h1, h2 with
   | Emp, Emp => true
@@ -89,7 +102,7 @@ Fixpoint eqheap h1 h2 :=
 
 Lemma eqheapP : Equality.axiom eqheap.
 Proof.
-elim=> [|n x tl IHh1 tr IHh2] [|m y h1 h2] /=; try by constructor.
+elim=> [|??? IHh1 ? IHh2] [|*] /=; try by constructor.
 by apply: (iffP and4P); case=> [/eqP-> /eqP-> /IHh1-> /IHh2->].
 Qed.
 
@@ -97,15 +110,6 @@ Canonical heap_eqMixin := EqMixin eqheapP.
 Canonical heap_eqType := Eval hnf in EqType (heap T) heap_eqMixin.
 
 Lemma eqheapE : eqheap = eq_op. Proof. by []. Qed.
-
-Lemma eqheap_Node (x1 x2 : T) n1 n2 tr1 tr2 tl1 tl2 :
-  ([tl1 | n1, x1 | tr1] == [tl2 | n2, x2 | tr2]) = [&& (n1 == n2), (x1 == x2), eqheap tl1 tl2 & eqheap tr1 tr2].
-Proof. by []. Qed.
-
-Lemma eqNode1xEE x y: ([ [||]| 1, x | [||]] == [ [||] | 1, y | [||]]) = (x == y).
-Proof.
-by rewrite eqheap_Node !eq_refl; case (x == y).
-Qed.
 
 Fixpoint mem_heap h :=
   if h is Node _ y tl tr then xpredU1 y (xpredU (mem_heap tl) (mem_heap tr)) else xpred0.
@@ -115,36 +119,12 @@ Identity Coercion heap_of_eqclass : heap_eqclass >-> heap.
 Coercion pred_of_heap (h : heap_eqclass) : {pred T} := mem_heap h.
 
 Canonical heap_predType := PredType pred_of_heap.
-(* The line below makes mem_seq a canonical instance of topred. *)
-Canonical mem_seq_predType := PredType mem_heap.
+(* The line below makes mem_heap a canonical instance of topred. *)
+Canonical mem_heap_predType := PredType mem_heap.
 
-Lemma in_Node x y n tl tr: 
+Lemma in_node x y n tl tr: 
   x \in [tl | n, y | tr] = [|| x == y, x \in tl | x \in tr].
 Proof. by []. Qed.
-(* Definition of count and simple properties *)
-Section Conut.
-Variables a : pred T.
-
-Fixpoint count h : nat := if h is [tl| _, x |tr] then a x + count
- tl + count tr else 0.
-
-Lemma count_Node tl tr y n: count [tl| n, y |tr] = a y + count tl + count tr.
-Proof. by []. Qed.
-
-Lemma count_E : count [||] = 0.
-Proof. by []. Qed.
-
-Lemma count_NodexEE n y : count [ [||]| n, y | [||]] = a y.
-Proof. move=> /=. by rewrite !addn0. Qed.
-
-Let countE := (count_Node, count_E, count_NodexEE).
-
-End Conut.
-
-Lemma in_count x h: x \in h = (0 < count (xpred1 x) h)%N.
-Proof.
-elim h=> // n y h1 IHh1 h2 IHh2; rewrite in_Node /= !addn_gt0 IHh1 IHh2 eq_sym; by case: (y == x).
-Qed.
 
 (* Definition of rank and size and simple properties *)
 Section Mesures.
@@ -156,10 +136,10 @@ Definition f1 (x y : nat) := y.+1.
 Lemma rank__NodexEE : f1 (rank [||]) (rank  [||]) = 1%N.
 Proof. by []. Qed.
 
-Lemma rankNode : forall tl tr n x, rank [tl| x, n |tr] = f1 (rank tl) (rank tr).
+Lemma rankNode tl tr n x : rank [tl| x, n |tr] = f1 (rank tl) (rank tr).
 Proof. by []. Qed.
 
-Lemma rank_Node_E : forall h1 h2 n x, (rank  [||] < rank [h1 | n, x | h2])%N.
+Lemma rank_Node_E h1 h2 n x : (rank  [||] < rank [h1 | n, x | h2])%N.
 Proof. by []. Qed.
 
 Fixpoint size h : nat :=
@@ -167,30 +147,131 @@ if h is Node _ _ a b then (size a) + (size b) + 1 else O.
 
 Definition f2 (x y : nat) := x + y + 1.
 
-Lemma sizeNode : forall tl tr n x, size [tl| x, n |tr] = f2 (size tl) (size tr).
+Lemma sizeNode tl tr n x : size [tl| x, n |tr] = f2 (size tl) (size tr).
 Proof. by []. Qed.
 
 Lemma size__NodexEE : f2 (size  [||]) (size  [||]) = 1%N.
 Proof. by []. Qed.
-
-Lemma size_Node_E : forall h1 h2 n x, (size  [||] < size [h1 | n, x | h2])%N.
-Proof. move=> /= h1 h2 n x. rewrite addn_gt0; apply/orP; by right. Qed.
-
-
-Lemma size_conut h : size =1 count xpredT.
-Proof. by elim=> //= n x h1 -> h2->; ssrnatlia. Qed.
+Lemma size_Node_E h1 h2 n x : (size  [||] < size [h1 | n, x | h2])%N.
+Proof. by rewrite addn_gt0 leqnn. Qed.
 
 End Mesures.
 
+(* Definition of count, all and simple properties *)
+Section HeapCount.
+Variables a : pred T.
 
-Definition empty h :=
-if h is Emp then true else false.
+Fixpoint count h : nat := if h is [tl| _, x |tr] then a x + count
+ tl + count tr else 0.
 
-Theorem emptyP h : reflect (h = Emp) (empty h).
-Proof. case h; by constructor. Qed.
+Lemma count_Node tl tr y n: count [tl| n, y |tr] = a y + count tl + count tr.
+Proof. by []. Qed.
 
+Lemma count_E : count [||] = 0.
+Proof. by []. Qed.
+
+Lemma count_NodexEE n y : count [[||]| n, y | [||]] = a y.
+Proof. by rewrite /= !addn0. Qed.
+
+Fixpoint all h := 
+if h is [tl| _, x |tr] then [&& a x, (all tl) & all tr] else true.
+
+End HeapCount.
+
+Lemma count_a_predT a h : (count a h <= count predT h)%N.
+Proof. elim: h=> //= n s *; case: (a s); by repeat apply: leq_add. Qed.
+Hint Resolve count_a_predT: core.
+
+Lemma size_count h : size =1 count predT.
+Proof. by elim=> //= n x h1 -> h2->; ssrnatlia. Qed.
+
+Lemma allE h a : reflect (count a h = size h) (all a h).
+Proof.
+rewrite size_count //.
+elim: h => /= [| _ s h1 /(sameP eqP) <- h2 /(sameP eqP) <-]; first by constructor.
+apply/introP => [/and3P[-> /eqP-> /eqP->]|] // H.
+suffices: ((a s) + count a h1 + count a h2 < 1 + count predT h1 + count predT h2)%N.
+- by move=> LE EQ; move: EQ LE=>->; rewrite ltnn.
+move: H=> /nandP[/negPf->|/nandP[] H] //=.
+- apply: add_lt_le=> //; apply : add_lt_le=> //.
+1: have: (count a h1 < count predT h1)%N=>*.
+3: have: (count a h2 < count predT h2)%N=>*.
+1,3: rewrite ltn_neqAle; apply/andP; by split.
+- apply: add_lt_le=> //; apply add_le_lt=> //; by case (a s).
+- apply: add_le_lt=> //. apply leq_add=> //; by case (a s).
+Qed.
+
+Lemma in_count x h: x \in h = (0 < count (xpred1 x) h)%N.
+Proof.
+elim h=> // n y h1 IHh1 h2 IHh2;
+by rewrite in_node /= !addn_gt0 IHh1 IHh2 eq_sym lt0b orbA.
+Qed.
+
+(* if h is heap oredered (see below) LE x h is same as   *)
+(* x is less or equal then all elements in heaps         *)
 Definition LE x h : bool := 
 if h is Node n y a b then (x <= y) else true.
+
+Lemma LE_trans y x h: LE y h -> (x <= y) -> LE x h.
+Proof. by case: h=> //= ???? H /le_trans/(_ H). Qed.
+
+(* Definition of heap ordered heaps and simpl properties *)
+Fixpoint heap_ordered h : bool :=
+if h is Node n x tl tr then
+  [&& (LE x tl), (LE x tr), (heap_ordered tl) & (heap_ordered tr)]
+else true.
+
+Lemma LE_correct h x y:
+heap_ordered h -> x \in h -> LE y h -> y <= x.
+Proof.
+by elim: h x y=> [| n x h1 IHh1 h2 IHh2 x' y' /= /and4P[L1 L2 H1 H2]] //
+/or3P[/eqP ->|/(IHh1 _ _ H1)/(_ L1)|/(IHh2 _ _ H2)/(_ L2)] // H /le_trans/(_ H).
+Qed.
+
+Lemma LE_spec x h : heap_ordered h ->
+  LE x h -> all (>= x) h.
+Proof.
+elim h=> // n y h1 IHh1 h2 IHh2 /= /and4P[???? XY].
+by rewrite XY IHh1 // ?IHh2 // ?(LE_trans y).
+Qed.
+
+Fact heap_ordered_NodexEE n x : heap_ordered [ [||]| n, x |  [||]].
+Proof. by []. Qed.
+Hint Resolve heap_ordered_NodexEE: core.
+Fact heap_ordered_E : heap_ordered [||]. Proof. by []. Qed.
+
+(* Some basic definitions for reasoning about spines in heaps *)
+Variant side := R | L.
+
+Definition spine := seq side.
+
+Fixpoint spine_in p h : bool :=
+match p, h with
+| R :: p, Node _ _ _ tr => spine_in p tr
+| L :: p, Node _ _ tl _ => spine_in p tl
+| [::],   Emp          => true
+| _,      _          => false
+end.
+
+Fixpoint right p : bool :=
+match p with
+| R :: p' => right p'
+| L :: _  => false
+| [::]    => true
+end.
+
+Lemma rigth_correct x s: right (x :: s) -> ((x = R) * right s).
+Proof. by case: s; case x. Qed.
+
+Lemma right_spine_ex h: exists s, right s && spine_in s h.
+Proof.
+elim: h=> [|n s hl _ hr [] s']; by [exists nil| exists (R :: s')].
+Qed.
+
+Lemma spine_in_E s : spine_in s Emp -> s = [::].
+Proof. by case: s=> [|[]] //=. Qed.
+
+(* Theory for heaps with leftist measure *)
 
 Section Measure.
 Variables measure : measureType T.
@@ -204,38 +285,16 @@ Hint Resolve measure_Node_E : core.
 Fixpoint measure_inv h : bool :=
 match h with
 | [tl| n, x |tr] => [&& (n == measure h), (measure_inv tl) & (measure_inv tr)]
-|  [||]            => true
+| [||]           => true
 end.
 
 Lemma measure_inv_NodexEE x : measure_inv [ [||]| measure1, x | [||]].
-Proof.
-  move=> /=. by rewrite measureNode measure_NodexEE eq_refl.
-Qed.
+Proof. by rewrite /= measureNode measure_NodexEE eq_refl. Qed.
 Hint Resolve measure_inv_NodexEE : core.
-
-Fixpoint heap_ordered h : bool :=
-if h is Node n x tl tr then
-  [&& (LE x tl), (LE x tr), (heap_ordered tl) & (heap_ordered tr)]
-else true.
-
-Lemma LE_trans y x h: LE y h -> (x <= y) -> LE x h.
-Proof. by case: h=> //= _ s _ _ H /le_trans/(_ H). Qed.
-
-
-Lemma LE_spec x h : heap_ordered h -> LE x h -> (count (>= x) h = count predT h).
-Proof.
-by elim h=> // n y h1 IHh1 h2 IHh2 /= /and4P[???? XY];
-rewrite XY IHh1 // ?IHh2 // ?(LE_trans y).
-Qed.
-
-
-Fact heap_ordered_NodexEE n x : heap_ordered [ [||]| n, x |  [||]].
-Proof. by []. Qed.
-Hint Resolve heap_ordered_NodexEE: core.
-Fact heap_ordered_E : heap_ordered [||]. Proof. by []. Qed.
 
 Fact measure_E : measure_inv [||]. Proof. by []. Qed.
 
+(* leftist invariant for arbitrary mesure and defonition of leftist heap *)
 Fixpoint leftist_inv h : bool :=
 if h is Node n x tl tr then
   [&& (measure tr <= measure tl)%N, (leftist_inv tl) & (leftist_inv tr)]
@@ -246,33 +305,6 @@ Proof. move=> /=; by rewrite leqnn. Qed.
 Hint Resolve leftist_inv_NodexEE : core.
 
 Fact leftist_inv_E : leftist_inv [||]. Proof. by []. Qed.
-
-Variant side := r | l.
-
-Definition spine := seq side.
-
-Fixpoint spine_in p h : bool :=
-match p, h with
-| r :: p, Node _ _ _ tr => spine_in p tr
-| l :: p, Node _ _ tl _ => spine_in p tl
-| [::],   Emp          => true
-| _,      _          => false
-end.
-
-Fixpoint Right p : bool :=
-match p with
-| r :: p' => Right p'
-| l :: _  => false
-| [::]    => true
-end.
-
-Lemma rigth_correct : forall x s, Right (x :: s) -> ((x = r) * Right s).
-Proof. move=> [] //=. Qed.
-
-Lemma case_spine_in : forall side s n x tl tr, 
-spine_in (side :: s) (Node n x tl tr) -> 
-if side is r then spine_in s tr else spine_in s tl.
-Proof. move=> [] //=. Qed.
 
 Definition leftist_measure_inv h := leftist_inv h && measure_inv h.
 
@@ -289,91 +321,18 @@ Proof.
 by rewrite /leftist_measure_inv => /andP[] /= => /and3P[->->-> /and3P[_ ->->]].
 Qed.
 
-Lemma case_measure_inv n y h1 h2 : 
-measure_inv (Node n y h1 h2) -> [&& (n == f (measure h1) (measure h2)), (measure_inv h1) & (measure_inv h2)].
-Proof. move=> /=; by rewrite measureNode. Qed.
-
 Lemma case_leftist_measure_inv n x tl tr: 
 leftist_measure_inv (Node n x tl tr) -> (n == f (measure tl) (measure tr)) &&
 [&& leftist_measure_inv tr, leftist_measure_inv tl & (measure tr <= measure tl)%N].
 Proof.
 move=> LI. move: LI (LI)=> /case_leftist_measure_inv_rl -> /andP[_] /= /and3P[]; 
 by rewrite measureNode=>->.
-Qed.
-
-Lemma case_heap_ordered n y h1 h2 : 
-heap_ordered (Node n y h1 h2) ->
-[&& LE y h1, LE y h2, (heap_ordered h1) & (heap_ordered h2)].
-Proof. by []. Qed.      
-
-
-Ltac merge_cases := match goal with 
-| H : (?x <= ?y) = true |- _ => move: (H)=> /= ->; rewrite ?H
-| H : (?x <= ?y) = false |- _ => move: (H)=> /merge_a /= ->; rewrite ?H
-end. 
-
-Ltac merge_casesxy x y := case H : (x <= y); merge_cases.
-Lemma swap_tact {A B C} : (A -> B -> C) -> (B -> A -> C).
-Proof.
-move=> H b /H; by apply.
-Qed.
-
-Ltac swapg := apply swap_tact.
-
-Lemma case_leftist_inv n y h1 h2 : 
-leftist_inv (Node n y h1 h2) -> [&& (measure h2 <= measure h1)%N, leftist_inv h1 & leftist_inv h2].
-Proof. by []. Qed.
-
-Lemma right_spine_ex : forall h, exists s, Right s && spine_in s h.
-Proof.
-elim=> [|n s hl _ hr [] s'].
-- by exists nil.
-by exists (r :: s').
-Qed.
-
-Lemma spine_in_E s : spine_in s Emp -> s = [::].
-Proof. by case: s=> [|[]] //=. Qed.
-
-Definition makeT (x : T) h1 h2 :=
-let m1 := measure h1 in
-  let m2 := measure h2 in
-      if (m2 <= m1)%N then [h1| f m1 m2, x |h2] else [h2| f m2 m1, x |h1] .
-
-Ltac makeT_cases := match goal with
-| H : (?a <= ?b)%N = _ |- _ => rewrite /makeT; move : H => /= ->
-end.
-
-Ltac makeT_casesxy x y := case fresh : (x <= y)%N; makeT_cases.
-
-Lemma makeT_preserves_LI_inv x tl tr :
-leftist_inv tl -> leftist_inv tr ->
-leftist_inv (makeT x tl tr).
-Proof. 
-rewrite /makeT; case: ifP=> H /=->->.
-- by rewrite H.
-- suffices: (measure tl <= measure tr)%N => [->|] //; move: H.
-move=> /neq0_lt0n; by ssrnatlia.
-Qed.
-
-Lemma makeT_preserves_rk_inv x tl tr :
-measure_inv tl -> measure_inv tr ->
-measure_inv (makeT x tl tr).
-Proof.
-by rewrite /makeT; case: ifP=> /= _ ->->; rewrite measureNode eq_refl. 
-Qed.
-
-Lemma makeT_peserves_HO_inv x tl tr :
-heap_ordered tl -> heap_ordered tr ->
-LE x tl -> LE x tr ->
-heap_ordered (makeT x tl tr).
-Proof.
-rewrite /makeT; by case: ifP => _ /=->->->->.
-Qed.
+Qed. 
 
 Definition leftistheap h :=
 [&& leftist_inv h, measure_inv h & heap_ordered h].
 
-Fact leftistheap_NodexEE x : leftistheap [ [||]| measure1, x |  [||]].
+Fact leftistheap_NodexEE x : leftistheap [[||]| measure1, x |[||]].
 Proof. by rewrite /leftistheap measure_inv_NodexEE heap_ordered_NodexEE leftist_inv_NodexEE. Qed.
 Hint Resolve leftistheap_NodexEE : core.
 
@@ -381,122 +340,41 @@ Fact leftistheap_E : leftistheap  [||].
 Proof. by rewrite /leftistheap. Qed.
 Hint Resolve leftistheap_E : core.
 
-Fixpoint merge a :=
-if a is Node n x a1 b1 then
-let fix merge_a b :=
-  if b is Node m y a2 b2 then
-    if x <= y then 
-      makeT x a1 (merge b1 b)
-    else
-      makeT y a2 (merge_a b2)
-  else a in
-merge_a
-else id.
+(* makeT takes two heaps and element and make heap from them *)
+(* with correct mesure                                       *)
+Definition makeT (x : T) h1 h2 :=
+let m1 := measure h1 in
+  let m2 := measure h2 in
+      if (m2 <= m1)%N then [h1| f m1 m2, x |h2] else [h2| f m2 m1, x |h1] .
 
-Arguments merge !tl !tr : rename.
-
-Lemma merge_E_h: forall h, merge Emp h = h.
-Proof.  by case. Qed.
-
-Lemma merge_h_E: forall h, merge h Emp = h.
-Proof. by case. Qed.
-
-Lemma measure_inv_r n x tl tr:
-measure_inv (Node n x tl tr) -> measure_inv tr.
-Proof. by move=> /and3P[]. Qed.
-
-Lemma measure_inv_l n x tl tr :
-measure_inv (Node n x tl tr) -> measure_inv tl.
-Proof. by move=> /and3P[]. Qed.
-
-Lemma merge_a nl nr x y tll tlr trr trl :
-(x <= y) = false -> 
-merge (Node nl x tll tlr) (Node nr y trl trr) = 
-makeT y trl (merge  (Node nl x tll tlr) trr).
-Proof.
-move=> /= ->.
-by elim: trr.
+Lemma makeT_LI_inv x tl tr :
+leftist_inv tl -> leftist_inv tr ->
+leftist_inv (makeT x tl tr).
+Proof. 
+rewrite /makeT; case: ifP=> H /=->->; first by rewrite H.
+- suffices: (measure tl <= measure tr)%N => [->|] //; move: H.
+move=> /neq0_lt0n; by ssrnatlia.
 Qed.
 
-Lemma merge_preserve_measure_inv : forall h1 h2,
-measure_inv h1 -> measure_inv h2 -> measure_inv (merge h1 h2) .
+Lemma makeT_rk_inv x tl tr :
+measure_inv tl -> measure_inv tr ->
+measure_inv (makeT x tl tr).
 Proof.
-elim=> [//| nl x tll IHhl tlr IHhr].
-elim=> [|nr y trl IH'hl trr IH'hr] //.
-merge_casesxy x y => /= /and3P[??? /and3P[*]];
-apply: makeT_preserves_rk_inv=> //; 
-[apply: IHhr|apply: IH'hr]=> //=; apply/and3P; by split.
+by rewrite /makeT; case: ifP=> /= _ ->->; rewrite measureNode eq_refl. 
 Qed.
 
-Lemma case_heap_ordered_l n x tl tr :
-heap_ordered (Node n x tl tr) -> (heap_ordered tl && LE x tl).
-Proof. by move=> /= /and4P[-> _ ->]. Qed.
-
-Lemma case_heap_ordered_r n x tl tr :
-heap_ordered (Node n x tl tr) -> (heap_ordered tr && LE x tr).
-Proof. by move=> /= /and4P[_ -> _ ->]. Qed.
-
-Lemma case_LE x y n tr tl :
-LE x (Node n y tl tr) -> x <= y.
-Proof. by []. Qed.
-
-Lemma merge_preserve_LE : forall h1 h2 x,
-LE x h1 -> LE x h2 -> LE x (merge h1 h2).
+Lemma makeT_peserve_HO_inv x tl tr :
+heap_ordered tl -> heap_ordered tr ->
+LE x tl -> LE x tr ->
+heap_ordered (makeT x tl tr).
 Proof.
-elim=> [//| nl x tll IHhl tlr IHhr].
-elim=> [|nr y trl IH'hl trr IH'hr x' /case_LE HH1 /case_LE HH2] //.
-by merge_casesxy x y;
-[makeT_casesxy (measure (merge tlr (Node nr y trl trr))) (measure tll)|
-  makeT_casesxy (measure (merge (Node nl x tll tlr) trr)) (measure trl)].
-Qed.
-
-Lemma merge_preserve_HO_inv : forall h1 h2,
-heap_ordered h1 -> heap_ordered h2 -> heap_ordered (merge h1 h2).
-Proof.
-elim=> [//| nl x tll IHhl tlr IHhr].
-elim=> [|nr y trl IH'hl trr IH'hr H1 H2] //.
-move : (H1) (H2)=>
-        /case_heap_ordered /and4P[L1 L2 HH1 HH2]
-        /case_heap_ordered /and4P[L'1 L'2 HH'1 HH'2] //;
-merge_casesxy x y; apply makeT_peserves_HO_inv=> //.
-1 : apply: IHhr=> //.
-2 : apply: IH'hr=> //.
-all : apply: merge_preserve_LE=> //=.
-move: (negbT H).
-by rewrite -ltNge lt_def=> /andP[_ ->].
-Qed.
-
-Lemma case_leftist_inv_l n x tl tr : leftist_inv (Node n x tl tr) -> leftist_inv tl.
-Proof. by move=> /and3P[].  Qed.
-
-Lemma case_leftist_inv_r n x tl tr : leftist_inv (Node n x tl tr) -> leftist_inv tr.
-Proof. by move=> /and3P[].  Qed.
-
-Lemma merge_preserve_LI_inv : forall h1 h2,
-leftist_inv h1 -> leftist_inv h2 -> leftist_inv (merge h1 h2).
-Proof.
-elim=> [//| nl x tll IHhl tlr IHhr].
-elim=> [|nr y trl IH'hl trr IH'hr H1 H2] //.
-move : (H1) (H2) =>  /and3P[_ HH1 HH2] /and3P[_ HH'1 HH'2].
-merge_casesxy x y; apply: makeT_preserves_LI_inv=> //.
-- by apply: IHhr.
-by apply: IH'hr.
-Qed.    
-
-Theorem merge_preserve_LH h1 h2 :
-leftistheap h1 -> leftistheap h2 -> leftistheap (merge h1 h2).
-Proof.
-move=> /and3P[LI1 RR1 HO1] /and3P[LI2 RR2 HO2]; apply/andP; split.
-- by apply: merge_preserve_LI_inv.
-- apply/andP; split.
-- by apply: merge_preserve_measure_inv.
-by apply: merge_preserve_HO_inv. 
+rewrite /makeT; by case: ifP => _ /=->->->->.
 Qed.
 
 Lemma makeT_spec h1 h2 x a: 
 count a (makeT x h1 h2) = a x + count a h1 + count a h2.
 Proof.
-by makeT_casesxy (measure h2) (measure h1)=> /=; ssrnatlia.
+rewrite /makeT; case: ifP=> /=; ssrnatlia.
 Qed.
 
 Lemma makeT_in_spec h1 h2 x y :
@@ -505,17 +383,95 @@ Proof.
 by rewrite !in_count makeT_spec eq_sym; case : (x == y)=> /=; rewrite !addn_gt0.
 Qed.
 
+(* fuction merge makes from two heaps nwe one that contains *)
+(* same elements (see merge_spec)                           *)
+(* Here your can see special total realization of merge     *)
+Fixpoint merge' a :=
+if a is Node n x a1 b1 then
+let fix merge_a b :=
+  if b is Node m y a2 b2 then
+    if x <= y then 
+      makeT x a1 (merge' b1 b)
+    else
+      makeT y a2 (merge_a b2)
+  else a in
+merge_a
+else id.
+
+Arguments merge' !tl !tr : rename.
+Definition merge := nosimpl merge'.
+
+Ltac merge_cases := match goal with 
+| H : (?x <= ?y) = true |- _ => move: (H); rewrite /merge /= =>->; rewrite ?H
+| H : (?x <= ?y) = false |- _ => move: (H)=> /merge_a /= ->; rewrite ?H
+end. 
+
+Ltac merge_casesxy x y := case H : (x <= y); merge_cases.
+
+Lemma merge_E_h h: merge Emp h = h.
+Proof. by []. Qed.
+
+Lemma merge_h_E h: merge h Emp = h.
+Proof. by case: h. Qed.
+
+Lemma merge_a nl nr x y tll tlr trr trl :
+(x <= y) = false -> 
+merge (Node nl x tll tlr) (Node nr y trl trr) = 
+makeT y trl (merge  (Node nl x tll tlr) trr).
+Proof. rewrite /merge /= => ->. by elim: trr. Qed.
+
+Lemma merge_measure_inv h1 h2:
+measure_inv h1 -> measure_inv h2 -> measure_inv (merge h1 h2) .
+Proof.
+elim: h1 h2=> // ? x ??? IHhr. elim=> // ? y ??? IH'hr.
+merge_casesxy x y => /= /and3P[??? /and3P[*]]; 
+apply: makeT_rk_inv=> //; 
+[apply: IHhr|apply: IH'hr]=> //=; apply/and3P; by split.
+Qed.
+
+Lemma merge_LE h1 h2 x:
+LE x h1 -> LE x h2 -> LE x (merge h1 h2).
+Proof.
+elim: h1 h2 x => // ? x ????. elim=> // ? y * /=.
+by merge_casesxy x y; rewrite /makeT; case: ifP.
+Qed.
+
+Lemma merge_HO_inv h1 h2:
+heap_ordered h1 -> heap_ordered h2 -> heap_ordered (merge h1 h2).
+Proof.
+elim: h1 h2=> // ? x ??? IHhr. elim=> // ? y ??? IH'hr H1 H2.
+move : (H1) (H2)=> /= /and4P[???? /= /and4P[????] //].
+merge_casesxy x y; apply makeT_peserve_HO_inv=> //;
+[apply: IHhr | | apply: IH'hr |]=> //; apply: merge_LE=> //=.
+move: (negbT H). by rewrite -ltNge lt_def=> /andP[_ ->].
+Qed.
+
+Lemma merge_LI_inv h1 h2:
+leftist_inv h1 -> leftist_inv h2 -> leftist_inv (merge h1 h2).
+Proof.
+elim: h1 h2=> // ? x ??? IHhr. elim=> // ? y ??? IH'hr H1 H2.
+move : (H1) (H2) => /and3P[??? /and3P[*]].
+merge_casesxy x y; apply: makeT_LI_inv=> //;
+by [apply: IHhr | apply: IH'hr].
+Qed.
+
+Theorem merge_LH h1 h2 :
+leftistheap h1 -> leftistheap h2 -> leftistheap (merge h1 h2).
+Proof.
+move=> /and3P[??? /and3P[*]]; apply/and3P; split;
+by [apply: merge_LI_inv |apply: merge_measure_inv|apply: merge_HO_inv]. 
+Qed.
+
 Theorem merge_spec h1 h2 a: 
   count a (merge h1 h2) = count a h1 + count a h2.
 Proof.
 elim: h1 h2=> [h2|n x h1 IHh1 h2 IHh2]; rewrite ?merge_E_h //.
 elim=> [/=|m y h21 IHh21 h22 IHh22]; first by ssrnatlia.
-- by merge_casesxy x y; rewrite makeT_spec; rewrite ?IHh2 ?IHh22 /=; ssrnatlia.
+by merge_casesxy x y; rewrite makeT_spec; rewrite ?IHh2 ?IHh22 /=; ssrnatlia.
 Qed.
 
 Lemma merge_size h1 h2 : size (merge h1 h2) = size h1 + size h2.
-Proof. by rewrite !size_conut ?merge_spec. Qed.
-
+Proof. by rewrite !size_count ?merge_spec. Qed.
 
 Theorem merge_in_spec  h1 h2 x :
 x \in (merge h1 h2) = ((x \in h1) || (x \in h2)).
@@ -523,153 +479,9 @@ Proof.
 by rewrite !in_count merge_spec !addn_gt0.
 Qed.
 
+(* Two defenition of insert, their equality and some properties *)
 Definition insert (x : T) h := 
 merge [[||]| measure1, x | [||]] h.
-
-
-Lemma insert_preserve_measure_inv : forall h x,
-measure_inv h -> measure_inv (insert x h).
-Proof.
-by move=> h x Rh; apply: merge_preserve_measure_inv.
-Qed.
-
-Lemma insert_preserve_HO_inv : forall h x,
-heap_ordered h -> heap_ordered (insert x h).
-Proof.
-by move=> h x Rh; apply: merge_preserve_HO_inv.
-Qed.
-
-Lemma insert_preserve_LI_inv : forall h x,
-leftist_inv h -> leftist_inv (insert x h).
-Proof.
-by move=> h x Rh; apply: merge_preserve_LI_inv.
-Qed.
-
-Theorem insert_preserve_LH : forall h x,
-leftistheap h -> leftistheap (insert x h).
-Proof.
-by move=> h x Rh; apply: merge_preserve_LH.
-Qed.
-
-Theorem insert_spec h x a : 
-  count a (insert x h) = a x + count a h.
-Proof. by rewrite merge_spec /=; ssrnatlia. Qed.
-
-Lemma insert_size h x: size (insert x h) = (size h).+1.
-Proof. by rewrite !size_conut ?merge_spec. Qed.
-
-
-Theorem insert_in_spec h x y :
-x \in (insert y h) = ((x == y) || (x \in h)).
-Proof.
-rewrite merge_in_spec /= !in_Node; case (x == y); by case (x \in h).
-Qed.
-
-Definition findmin h := 
-if h is Node _ x _ _ then Some x else None.
-
-Theorem findmin_correct1 : forall h,
-None = findmin h <-> h = Emp.
-Proof. split=> [|-> //]. by case : h. Qed.
-
-Lemma LE_correct : forall h x y,
-heap_ordered h -> x \in h -> LE y h -> y <= x.
-Proof.
-elim=> [x y _ H| n x h1 IHh1 h2 IHh2 x' y' /= /and4P[L1 L2 H1 H2]] //
- /or3P[/eqP ->|/(IHh1 _ _ H1)/(_ L1)|/(IHh2 _ _ H2)/(_ L2)] //; swapg; exact: le_trans.
-Qed.
-
-Theorem findmin_correct2 : forall h, heap_ordered h ->
-forall z, Some z = findmin h -> forall x, x \in h -> z <= x.
-Proof.
-case=> [//| n x h1 h2 HO z /= [->] y /or3P[/eqP ->||]] // H. 
-- by move: HO=> /case_heap_ordered_l /andP[/LE_correct - /(_ _ x H)].
-by move: HO=> /case_heap_ordered_r /andP[/LE_correct - /(_ _ x H)].
-Qed.
-
-Lemma findmin_cases : forall h, (exists x, Some x = findmin h) \/ (h = Emp).
-Proof.
-case=> [|n z h1 h2 /=]; first by right.
-by left; exists z.
-Qed.
-
-Theorem findmin_LE_correct : forall x h,
-heap_ordered h ->
-((x \in h) && LE x h) <-> (Some x = findmin h).
-Proof.
-split=> [/andP[]|]; move: h H=> [] //.
-- move=> n y h1 h2 /= /and4P[L1 L2 H1 H2]
-  /or3P[/eqP-> //|/(LE_correct _ _ _ H1)/(_ L1)|/(LE_correct _ _ _ H2)/(_ L2)] XY YX;
-  suffices: x = y=> [-> //|]; apply: le_anti; rewrite XY YX //.
-move=> n s h1 h2 HO [] ->; apply/andP; split=> //=. 
-by rewrite in_Node eq_refl.
-Qed.
-
-Definition deletemin h :=
-if h is Node _ _ a b then merge a b else Emp.
-
-Lemma measure_inv_eq n x h1 h2 :
-measure_inv (Node n x h1 h2) -> n = f (measure h1) (measure h2).
-Proof. by move=> /= /and3P[/eqP]; rewrite measureNode. Qed.
-
-Lemma case_LE' x y h1 h2 n :
-LE x (Node n y h1 h2) -> ((x <= y) = true).
-Proof. by move=> /= ->. Qed.
-
-Lemma case_leftistheap_l n x h1 h2 :
-leftistheap (Node n x h1 h2) -> leftistheap h1.
-Proof.
-by rewrite /leftistheap=> /and3P[/case_leftist_inv_l-> /=/and3P[_ -> _] /and4P[]].
-Qed.
-
-Lemma case_leftistheap_r n x h1 h2 :
-leftistheap (Node n x h1 h2) -> leftistheap h2.
-Proof. 
-by rewrite /leftistheap=> /and3P[/case_leftist_inv_r-> /=/and3P[_ _ -> /and4P[]]].
-Qed.
-
-Lemma deletemin_preserve_rk_inv : forall h, 
-measure_inv h -> measure_inv (deletemin h).
-Proof.
-by case=> //=n x h1 h2 H; apply merge_preserve_measure_inv; move: H=> /and3P[].
-Qed.
-
-Lemma deletemin_preserve_HO_inv : forall h, 
-heap_ordered h -> heap_ordered (deletemin h).
-Proof.
-case=> //=n x h1 h2 H; apply merge_preserve_HO_inv; by move: H=> /and4P[].
-Qed.
-
-Lemma deletemin_preserve_LI_inv : forall h, 
-leftist_inv h -> leftist_inv (deletemin h).
-Proof.
-by case=> //=n x h1 h2 H; apply merge_preserve_LI_inv; move: H=> /and3P[].
-Qed.
-
-Lemma deletemin_correct : forall h, 
-leftistheap h -> leftistheap (deletemin h).
-Proof.
-case=> //=n x h1 h2 H; apply merge_preserve_LH; move: H.
-- by move/case_leftistheap_l.
-by move/case_leftistheap_r.
-Qed.
-
-Theorem deletemin_spec h x: 
-  Some x = findmin h -> (count^~ (insert x (deletemin h)) =1 count^~ h).
-Proof.
-by case: h=> // n y h1 h2 /= [->] a; rewrite insert_spec merge_spec addnA.
-Qed.
-
-Lemma deletemin_size h : size (deletemin h) = (size h).-1.
-Proof. case: h=> // n x tl tr; by rewrite ?size_conut //= merge_spec. Qed.
-
-
-Theorem deletemin_in_spec : forall h x y,
-Some x = findmin h -> (y \in (insert x (deletemin h))) = (y \in h).
-Proof.
-case=> [//=|n x h1 h2 y z [->]].
-by rewrite insert_in_spec /deletemin merge_in_spec //= orbA.
-Qed.
 
 Fixpoint insert' (x : T) h :=
 if h is Node n y a b then
@@ -679,19 +491,121 @@ let h' := Node n y a b in
   else makeT y a (insert' x b)
 else Node measure1 x Emp Emp.
 
+Lemma insert_measure_inv h x: measure_inv h -> measure_inv (insert x h).
+Proof. by move=> *; apply: merge_measure_inv. Qed.
+
+Lemma insert_HO_inv h x: heap_ordered h -> heap_ordered (insert x h).
+Proof. by move=> *; apply: merge_HO_inv. Qed.
+
+Lemma insert_LI_inv h x: leftist_inv h -> leftist_inv (insert x h).
+Proof. by move=> *; apply: merge_LI_inv. Qed.
+
+Theorem insert_LH h x: leftistheap h -> leftistheap (insert x h).
+Proof. by move=> *; apply: merge_LH. Qed.
+
+Theorem insert_spec h x a : count a (insert x h) = a x + count a h.
+Proof. by rewrite merge_spec /=; ssrnatlia. Qed.
+
+Lemma insert_size h x: size (insert x h) = (size h).+1.
+Proof. by rewrite !size_count ?merge_spec. Qed.
+
 Theorem insertE x h : measure_inv h -> leftist_inv h -> insert' x h = insert x h.
 Proof.
 rewrite /insert.
-elim h=> [//|n y h1 IHh1 h2 IHh2 MI LI] //.
-merge_casesxy x y=> //; rewrite ?IHh2 //.
-- rewrite /makeT.
-  have: (measure [h1 | n, y | h2] <= measure [||] = false)%N.
-- by apply/negbTE; rewrite -ltnNge. 
-- by move=>->.
-- by move: MI=> /= /and3P[].
-by move: LI=> /= /and3P[].
+elim h=> // n y h1 IHh1 h2 IHh2 /= /and3P[??? /and3P[*]].
+merge_casesxy x y=> //; rewrite ?IHh2 // /makeT.
+have: (measure [h1 | n, y | h2] <= measure [||] = false)%N=> [|->] //.
+by apply/negbTE; rewrite -ltnNge. 
 Qed.
 
+Theorem insert_in_spec h x y :
+x \in (insert y h) = ((x == y) || (x \in h)).
+Proof. 
+rewrite merge_in_spec /= !in_node; case (x == y); by case (x \in h).
+Qed.
+
+
+(* Properties of findmin function *)
+Definition findmin h := 
+if h is Node _ x _ _ then Some x else None.
+
+Theorem findmin_None h:
+None = findmin h <-> h = [||].
+Proof. split=> [|-> //]. by case : h. Qed.
+
+Theorem findmin_Some h z: heap_ordered h ->
+Some z = findmin h -> all (>= z) h.
+Proof. 
+case: h=> //= _ ??? /and3P[?? /andP[?? [->]]]; by rewrite lexx ?LE_spec. 
+Qed.
+
+Lemma findmin_cases h: (exists x, Some x = findmin h) \/ (h = Emp).
+Proof. case: h=> [|n z h1 h2 /=]; first by right. by left; exists z. Qed.
+
+Theorem findmin_spec x h:
+heap_ordered h ->
+((x \in h) && LE x h) <-> (Some x = findmin h).
+Proof.
+split=> [/andP[]|]; move: h H=> [] //.
+- move=> n y h1 h2 /= /and4P[L1 L2 H1 H2]
+  /or3P[/eqP-> //|/(LE_correct _ _ _ H1)/(_ L1)|/(LE_correct _ _ _ H2)/(_ L2)] XY YX;
+suffices: x = y=> [-> //|]; apply: le_anti; rewrite XY YX //.
+move=> ????? [->]; apply/andP; split=> //=. by rewrite in_node eq_refl.
+Qed.
+
+(* Properties of findmin function *)
+Definition deletemin h :=
+if h is Node _ _ a b then merge a b else Emp.
+
+Lemma case_leftistheap n x h1 h2 :
+leftistheap (Node n x h1 h2) -> leftistheap h1 && leftistheap h2.
+Proof.
+by rewrite/leftistheap=>/and3P[/=/and3P[_->->/=/and3P[_->->/and4P[_ _->->]]]].
+Qed.
+
+Lemma deletemin_rk_inv h:
+measure_inv h -> measure_inv (deletemin h).
+Proof.
+by case: h=> //=n x h1 h2 H; apply merge_measure_inv; move: H=> /and3P[].
+Qed.
+
+Lemma deletemin_HO_inv h:
+heap_ordered h -> heap_ordered (deletemin h).
+Proof.
+case: h=> //=n x h1 h2 H; apply merge_HO_inv; by move: H=> /and4P[].
+Qed.
+
+Lemma deletemin_LI_inv h:
+leftist_inv h -> leftist_inv (deletemin h).
+Proof.
+by case: h=> //=n x h1 h2 H; apply merge_LI_inv; move: H=> /and3P[].
+Qed.
+
+Lemma deletemin_correct h:
+leftistheap h -> leftistheap (deletemin h).
+Proof.
+by case: h=> //=???? H; apply merge_LH; move: H=> /case_leftistheap/andP[].
+Qed.
+
+Theorem deletemin_spec h x: 
+  Some x = findmin h -> (count^~ (insert x (deletemin h)) =1 count^~ h).
+Proof. by case: h=>// ????/= [->?]; rewrite insert_spec merge_spec addnA. Qed.
+
+Lemma deletemin_size h : size (deletemin h) = (size h).-1.
+Proof. case: h=> // n x tl tr; by rewrite ?size_count //= merge_spec. Qed.
+
+Theorem deletemin_in_spec h x y:
+Some x = findmin h -> (y \in (insert x (deletemin h))) = (y \in h).
+Proof.
+case: h=> // ???? [->].
+by rewrite insert_in_spec /deletemin merge_in_spec // orbA.
+Qed.
+
+(* In this section we define heapsort and prove it's properties *)
+(* heapsort fist translates sequense of elements into heap and  *)
+(* than takes the minimal element of the heap while it is not   *)
+(* empty                                                        *)
+Section Heapsort.
 Implicit Type hh : seq (option (heap T)).
 
 Fixpoint seq_to_seqheap (st : seq T) :=
@@ -709,10 +623,12 @@ Fixpoint count_seq a (sh : seq (heap T)) :=
   if sh is h :: sh' then count a h + count_seq a sh' else 0.
 
 Theorem seq_to_seqheap_spec s: count_seq^~ (seq_to_seqheap s) =1 seq.count^~ s.
-Proof.
-move=> a; elim: s=> //= x s->; ssrnatlia.
-Qed.
+Proof. move=> a; elim: s=> //= x s->; ssrnatlia. Qed.
 
+(* Now we want to define fromseq function that will translate  *)
+(* sequense of elements into heap in O(n) time                 *)
+(* Our implementation is based on divide and conqure principle *)
+(* adapted to total languages                                  *)
 Fixpoint fromseqheap_push h1 hh :=
   match hh with
   | None :: hh' | [::] as hh' => (some h1) :: hh'
@@ -721,7 +637,7 @@ Fixpoint fromseqheap_push h1 hh :=
 
 Fixpoint fromseqheap_pop h1 hh :=
   if hh is sh2 :: hh' then
-    let h2 := if sh2 is some h then h else   [||] in
+    let h2 := if sh2 is some h then h else [||] in
    fromseqheap_pop (merge h2 h1) hh' else h1.
 
 Fixpoint fromseqheap_rec hh sh  :=
@@ -729,7 +645,7 @@ Fixpoint fromseqheap_rec hh sh  :=
   | [:: x1, x2 & h'] => let h1 := merge x1 x2 in
     fromseqheap_rec (fromseqheap_push h1 hh) h'
   | [:: h] => fromseqheap_pop h hh
-  | [::] => fromseqheap_pop (  [||]) hh
+  | [::] => fromseqheap_pop [||] hh
   end.
 
 Definition fromseqheap := (fromseqheap_rec [::]).
@@ -758,7 +674,6 @@ Proof.
 elim: hh=> [|[sh|] hh' IHhh] //= in h *. by rewrite IHhh merge_spec; ssrnatlia.
 Qed.
 
-
 Lemma fromseqheap_rec1_spec sh hh a: 
   count a (fromseqheap_rec1 hh sh) = count_sseq a hh + count_seq a sh.
 Proof.
@@ -768,9 +683,7 @@ Qed.
 
 Lemma fromseqheap_spec sh : 
  count^~ (fromseqheap sh) =1 count_seq^~ sh.
-Proof.
-move=> a; by rewrite fromseqheapE fromseqheap_rec1_spec.
-Qed.
+Proof. move=> a; by rewrite fromseqheapE fromseqheap_rec1_spec. Qed.
 
 Theorem fromseq_cspec (s : seq T): 
   seq.count^~ s =1 count^~ (fromseq s).
@@ -778,12 +691,14 @@ Proof.
 move=> a; by rewrite /fromseq /= fromseqheap_spec seq_to_seqheap_spec.
 Qed.
 
+(* In this section we prove that fromseq s statisfy any invariant *)
+(* with spesial properties                                        *)
 Section Invariant.
 Definition invariant := heap T -> bool.
 
 Variables inv : invariant.
 
-Hypothesis merge_preserve_invariat : forall h1 h2, inv h1 -> inv h2 -> inv (merge h1 h2).
+Hypothesis merge_invariat : forall h1 h2, inv h1 -> inv h2 -> inv (merge h1 h2).
 Hypothesis inv_E : inv [||].
 Hypothesis inv_NodexEE : forall x, inv [[||]| measure1, x |  [||]].
 Hint Resolve inv_E : core.
@@ -791,22 +706,22 @@ Hint Resolve inv_E : core.
 Definition some_inv sh := if sh is some h then inv h else true.
 
 Lemma inv_fromseqheap_pop h sh: 
-  (all some_inv sh) -> inv h -> inv (fromseqheap_pop h sh).
+  (seq.all some_inv sh) -> inv h -> inv (fromseqheap_pop h sh).
 Proof.
 elim: sh => [|[h'|] shh IHhh] //= in h *=> /andP[HH' ASH HH]; apply: IHhh=> //.
-by apply: merge_preserve_invariat.
+by apply: merge_invariat.
 Qed.
 
 Lemma all_inv_fromseqheap_push h hh:
-  inv h -> (all some_inv hh) ->
-  all some_inv (fromseqheap_push h hh) = (inv h) && (all some_inv hh).
+  inv h -> (seq.all some_inv hh) ->
+  seq.all some_inv (fromseqheap_push h hh) = (inv h) && (seq.all some_inv hh).
 Proof.
 by elim: hh=> [|[sh|] hh' IHhh] //= in h *=> HH /andP[SH AHH];
- rewrite IHhh ?merge_preserve_invariat // HH SH.
+rewrite IHhh ?merge_invariat // HH SH.
 Qed.
 
 Lemma inv_fromseqheap_rec1 hh sh : 
-(all some_inv  hh) -> (all inv sh) -> (inv (fromseqheap_rec1 hh sh)).
+(seq.all some_inv  hh) -> (seq.all inv sh) -> (inv (fromseqheap_rec1 hh sh)).
 Proof.
 elim: sh => [|h sh IHsh] /= in hh *=> AHH; rewrite ?inv_fromseqheap_pop //.
 move=> /andP[HH AHS]. by apply: IHsh; rewrite ?all_inv_fromseqheap_push ?HH ?AHS ?AHH.
@@ -814,19 +729,15 @@ Qed.
 
 
 Lemma inv_fromseqheap sh : 
-all inv sh -> inv (fromseqheap sh).
-Proof.
-move=> ASH; by rewrite fromseqheapE inv_fromseqheap_rec1.
-Qed.
+seq.all inv sh -> inv (fromseqheap sh).
+Proof. move=> ASH; by rewrite fromseqheapE inv_fromseqheap_rec1. Qed.
 
 Lemma all_inv_seq_toseqheap s : 
-all inv (seq_to_seqheap s).
+seq.all inv (seq_to_seqheap s).
 Proof. elim: s=> //= a h->; by rewrite inv_NodexEE. Qed.
 
 Lemma inv_fromseq s : inv (fromseq s).
-Proof.
-by rewrite /fromseq /= inv_fromseqheap // all_inv_seq_toseqheap.
-Qed.
+Proof. by rewrite /fromseq /= inv_fromseqheap // all_inv_seq_toseqheap. Qed.
 End Invariant.
 
 Lemma measure_inv_E : measure_inv [||].
@@ -834,16 +745,16 @@ Proof. by []. Qed.
 
 
 Definition rank_rk_fromseq : forall s, measure_inv (fromseq s) := 
-  inv_fromseq measure_inv merge_preserve_measure_inv measure_inv_E measure_inv_NodexEE.
+  inv_fromseq measure_inv merge_measure_inv measure_inv_E measure_inv_NodexEE.
 
 Definition heap_ordered_fromseq : forall s, heap_ordered (fromseq s) := 
-  inv_fromseq heap_ordered merge_preserve_HO_inv heap_ordered_E (heap_ordered_NodexEE measure1).
+  inv_fromseq heap_ordered merge_HO_inv heap_ordered_E (heap_ordered_NodexEE measure1).
 
 Definition leftist_inv_fromseq : forall s, leftist_inv (fromseq s) := 
-  inv_fromseq leftist_inv merge_preserve_LI_inv leftist_inv_E (leftist_inv_NodexEE measure1).
+  inv_fromseq leftist_inv merge_LI_inv leftist_inv_E (leftist_inv_NodexEE measure1).
 
 Definition leftistheap_fromseq : forall s, leftistheap (fromseq s) := 
-  inv_fromseq leftistheap merge_preserve_LH leftistheap_E leftistheap_NodexEE.
+  inv_fromseq leftistheap merge_LH leftistheap_E leftistheap_NodexEE.
 
 
 Equations fromheap h : seq T by wf (size h) lt:=
@@ -861,13 +772,13 @@ Qed.
 Lemma fromheap_srec1_in x h: (x \in h) = (x \in (fromheap h)).
 Proof. by rewrite !in_count -has_pred1 has_count -fromheap_spec1. Qed.
 
-Search _ seq.size seq.count.
-
 Lemma fromheap_spec2 h: (heap_ordered h) -> sorted <=%O (fromheap h).
 Proof.
-apply_funelim (fromheap h)=> //= _ x h1 h2 IHh /and4P[*];
-  rewrite path_sortedE ?IHh ?all_count -?count_predT -?fromheap_spec1 ?merge_spec ?LE_spec ?eq_refl //.
-- by apply: merge_preserve_HO_inv.
+apply_funelim (fromheap h)=> //= _ x h1 h2 IHh /and4P[L1 L2 H1 H2];
+rewrite path_sortedE ?IHh ?all_count -?count_predT -?fromheap_spec1 ?merge_spec.
+by rewrite (allE _ _ (LE_spec _ _ H1 L1)) (allE _ _ (LE_spec _ _ H2 L2))
+ !size_count // eq_refl.
+- by apply: merge_HO_inv.
 by exact le_trans.
 Qed.
 
@@ -881,7 +792,7 @@ Proof. move=> p. by rewrite /heapsort -fromheap_spec1 fromseq_cspec. Qed.
 
 Theorem perm_heapsort s : perm_eql (heapsort s) s.
 Proof. apply/permPl/permP; by apply: count_heapsort. Qed.
-
+End Heapsort.
 End Measure.
 
 Definition rank_measureMixin : Measure.mixin_of rank := Measure.Mixin T rank 1%N f1 rankNode rank__NodexEE rank_Node_E.
@@ -895,9 +806,6 @@ Definition case_leftist_rank_inv := (case_leftist_measure_inv rank_measureType).
 Definition case_leftist_rank_inv_r := (case_leftist_measure_inv_r rank_measureType).
 Definition case_leftist_rank_inv_rl := (case_leftist_measure_inv_rl rank_measureType).
 
-Lemma rank_correct x n tl tr : measure_inv rank_measureType [tl| n, x |tr] -> n == (rank tr).+1.
-Proof. by move=> /= /and3P[]. Qed.
-
 Section Grank.
 
 (** The (general) rank of a tree is the length of the shortest path from the root to leaves *)
@@ -908,40 +816,39 @@ Fixpoint grank h : nat :=
 
 Theorem grank_rk h : leftist_rank_inv  h -> grank h = rank h.
 Proof.
-elim: h=> // n x h1 IHh1 h2 IHh2
-          /case_leftist_rank_inv/andP[]. rewrite /f /= /f1=>_ /and3P[L1 L2].
+elim: h=> // ??? IHh1 ? IHh2 /case_leftist_rank_inv/andP[].
+rewrite /f /= /f1=>_ /and3P[??].
 rewrite IHh1 // IHh2 //. by rewrite minnC ?Order.NatOrder.minnE=> ->.
 Qed.
 
 End Grank.
 
+(* We can obtain that right spine is the shoterst for heaps with *)
+(* rank measure                                                  *)
 Section Spine.
 
-Lemma length_right_spine : forall h s, 
-leftist_rank_inv h -> Right s -> spine_in s h -> length s = rank h.
+Lemma length_right_spine h s:
+leftist_rank_inv h -> right s -> spine_in s h -> length s = rank h.
 Proof.
-move=> h s /andP [] _ RC.
-elim: h s RC=> 
-[[|[]]|n x tl IHhl tr IHtr [_ _|[s /= /and3P[_ RRl RRr] |]]] //= R S.
-apply/eqnP=> /=. apply/eqP. by apply: IHtr.
+move=> /andP[_ RC].
+elim: h s RC=> [[|[]]|????? IHtr [_ _|[s /= /and3P[_ *]|]]] //.
+apply/eqnP=> /=; apply/eqP. by apply: IHtr.
 Qed.
 
-Theorem rigth_spine_shortest : 
-forall H s1 s2, Right s1 -> leftist_rank_inv H -> spine_in s1 H -> spine_in s2 H ->
+Theorem rigth_spine_shortest H s1 s2:
+ right s1 -> leftist_rank_inv H -> spine_in s1 H -> spine_in s2 H ->
 (length s1 <= length s2)%nat.
 Proof. 
-elim=>
-[s1 s2 _ _ /spine_in_E->|
-n x tl IHtl tr IHtr [//|
-a s1 [ _ _ _ |[]
-s2 /rigth_correct [] ->]]] //= => [Rs1 /case_leftist_rank_inv_r LI|
-Rs1 /case_leftist_rank_inv_rl /and3P[LI1 LI2 LE]] => SI1 SI2.
+elim: H s1 s2=>
+[???? /spine_in_E->|?? tl IHtl tr IHtr [//|a s1 [??? |[]
+s2 /rigth_correct [] ->]]] //= => [? /case_leftist_rank_inv_r ?|
+? /case_leftist_rank_inv_rl /and3P[??/=?]]=>*.
 - rewrite -addn1 -[(length s2).+1]addn1 leq_add2r. by apply IHtr.
 rewrite (length_right_spine tr s1) //.
-case: (right_spine_ex tl)=> s /andP [] Rs SIstl.
-suffices: (rank tl <= length s2)%N. move: LE=> /=; ssrnatlia.
+case: (right_spine_ex tl)=> s /andP[*].
+suffices: (rank tl <= length s2)%N; first by ssrnatlia.
 rewrite -(length_right_spine tl s) //.
-apply: IHtl=> //.
+by apply: IHtl.
 Qed.
 End Spine.
 End Specifications.
